theories/lang/notations.v
@@ -8,23 +8,43 @@ Notation Fail := (App #() #())
 ( only parsing
 ).
 
-Notation "e .0" := (e +ₗ #0%Z)%E
+Notation "e .(0)" := (e +ₗ 0%Z)%stdpp
 ( at level 2,
   left associativity,
-  format "e .0"
+  format "e .(0)"
+) : stdpp_scope.
+Notation "e .(1)" := (e +ₗ 1%Z)%stdpp
+( at level 2,
+  left associativity,
+  format "e .(1)"
+) : stdpp_scope.
+Notation "e .(2)" := (e +ₗ 2%Z)%stdpp
+( at level 2,
+  left associativity,
+  format "e .(2)"
+) : stdpp_scope.
+Notation "e .(3)" := (e +ₗ 3%Z)%stdpp
+( at level 2,
+  left associativity,
+  format "e .(3)"
+) : stdpp_scope.
+Notation "e .(0)" := (e +ₗ #0%Z)%E
+( at level 2,
+  left associativity,
+  format "e .(0)"
 ) : expr_scope.
-Notation "e .1" := (e +ₗ #1%Z)%E
+Notation "e .(1)" := (e +ₗ #1%Z)%E
 ( at level 2,
   left associativity,
-  format "e .1"
+  format "e .(1)"
 ) : expr_scope.
-Notation "e .2" := (e +ₗ #2%Z)%E
+Notation "e .(2)" := (e +ₗ #2%Z)%E
 ( at level 2,
   left associativity,
-  format "e .2"
+  format "e .(2)"
 ) : expr_scope.
-Notation "e .3" := (e +ₗ #3%Z)%E
+Notation "e .(3)" := (e +ₗ #3%Z)%E
 ( at level 2,
   left associativity,
-  format "e .3"
+  format "e .(3)"
 ) : expr_scope.
